QuickSortInLean/QuickSortPermutation.lean
@@ -1,53 +1,74 @@
 import QuickSortInLean.Permutation
 import QuickSortInLean.QuickSort
 
--- NOTE: somehow we need to write ∃_ : permuted arr arr', True instead of permuted arr arr'.
--- Otherwise, split tactic will not work.
-theorem partition'_permutation [Ord α] :
-  (partition' (arr : Array α) i j last ij jl la).2 = arr' → ∃_ : permuted arr arr', True := by
-  unfold partition'
-  split <;> simp [dbgTraceIfShared]
-  case inl jl =>
-    split
-    -- | .lt | .eq
-    case h_1 | h_2 =>
-      intro eq
-      let ⟨ih, _⟩ := partition'_permutation eq
-      exact ⟨.step _ _ ih, trivial⟩
-    -- | .gt
-    case h_3 =>
-      intro eq
-      exact partition'_permutation eq
-  case inr _ =>
-    intro eq
-    rw [←eq]
-    exact ⟨.step _ _ .refl, trivial⟩
-termination_by partition'_permutation α arr i j last ij jl la result ord => last - j
+theorem partitionImpl_permuted {α : Type} [Ord α]
+  {n : Nat} (arr : Vec α n) (first i j : Nat)
+  (fi : first ≤ i) (ij : i ≤ j) (jn : j < n) :
+  permuted n arr (partitionImpl arr first i j fi ij jn).2 := by
+  -- Constants
+  have : first < n := Nat.lt_of_le_of_lt (Nat.le_trans fi ij) jn
+  have : i < n := Nat.lt_of_le_of_lt ij jn
+  have : i - 1 ≤ j - 1 := Nat.sub_le_sub_right ij 1
+  have : j - 1 < n := Nat.lt_of_le_of_lt (Nat.sub_le ..) jn
+  let i' : Fin n := ⟨i, by assumption⟩
+  let j' : Fin n := ⟨j, jn⟩
 
-theorem partition_permutation [Ord α] :
-  (partition (arr : Array α) first last jl la).2 = arr' → ∃_ : permuted arr arr', True := by
-    simp [partition]
-    exact partition'_permutation
+  -- Proof
+  unfold partitionImpl
+  match Nat.decLt first i with
+  | isTrue h =>
+    have : first ≤ i - 1 := Nat.le_sub_of_lt h
+    simp [h, dbgTraceIfShared]
+    match hm : compare arr[i] arr[first] with
+    | .lt =>
+      simp [hm]
+      apply partitionImpl_permuted
+    | .eq | .gt =>
+      simp [hm]
+      show permuted n arr (partitionImpl (arr.swap i' j') first (i - 1) (j - 1) _ _ _).2
+      let ih := partitionImpl_permuted (arr.swap i' j') first (i - 1) (j - 1) (by assumption) (by assumption) (by assumption)
+      apply permuted.step i' j' ih
+  | isFalse h =>
+    simp [h, dbgTraceIfShared]
+    exact .step ⟨first, by assumption⟩ j' .refl
 
--- TODO: It's really hard to see through the definition of quickSort'.
-theorem quickSort'_permutation [Ord α] :
-  (quickSort' (arr : Array α) first last la).val = arr' → ∃_ : permuted arr arr', True := by
-  sorry
+theorem partition_permuted {α : Type} [Ord α]
+  {n : Nat} (arr : Vec α n) (first last : Nat)
+  (fl : first ≤ last) (ln : last < n) :
+  permuted n arr (partition arr first last fl ln).2 := by
+  apply partitionImpl_permuted
 
-theorem quickSort_permutation [Ord α] :
-  (quickSort (arr : Array α)) = arr' → ∃_ : permuted arr arr', True := by
-  simp [quickSort]
-  split
-  case inl => exact quickSort'_permutation
-  case inr =>
-    intro eq
-    rw [eq]
-    exact ⟨.refl, trivial⟩
+theorem quickSortImpl_permuted {α : Type} [Ord α]
+  {n : Nat} (arr : Vec α n) (first last : Nat) (ln : last < n) :
+  permuted n arr (quickSortImpl arr first last ln) := by
+  unfold quickSortImpl
+  match Nat.decLt first last with
+  | isTrue h =>
+    have : first ≤ last := Nat.le_of_lt h
 
-theorem quickSort_map_index_invertible {arr arr' : Array α} [Ord α] :
-  quickSort arr = arr' →
-  ∃f : Fin arr.size → Fin arr'.size,
-    invertible f ∧ (∀i : Fin arr.size, arr[i] = arr'[f i]) := by
-  intro eq
-  let ⟨p, _⟩ := quickSort_permutation eq
-  exact permuted_map_index_invertible p
+    simp [h]
+    sorry -- RAGE QUIT
+  | isFalse h =>
+    simp [h]
+    exact .refl
+termination_by _ => last - first
+
+theorem quickSort'_permuted {α : Type} [Ord α] {n : Nat} (arr : Vec α n) :
+  permuted n arr (quickSort' arr) := by
+  simp [quickSort']
+  match Nat.decLt 0 n with
+  | isTrue h =>
+    simp [h]
+    apply quickSortImpl_permuted arr
+  | isFalse h =>
+    simp [h]
+    exact .refl
+
+theorem quickSort'_map_index_invertible {α : Type} [Ord α] {n : Nat} (arr : Vec α n):
+  ∃f : Fin n → Fin n,
+    invertible f ∧ (∀i : Fin n, arr[i] = (quickSort' arr)[f i]) := by
+  let p := quickSort'_permuted arr
+  exists p.to_map
+  apply And.intro
+  . exact permuted_map_invertible p
+  . exact permuted_map_index p
